modernized examples; removed now trivial "HFset"

src/HOL/BNF/Examples/Lambda_Term.thy
@@ -15,203 +15,57 @@ begin
 
 section {* Datatype definition *}
 
-data_raw trm: 'trm = "'a + 'trm \<times> 'trm + 'a \<times> 'trm + ('a \<times> 'trm) fset \<times> 'trm"
+data 'a trm =
+  Var 'a |
+  App "'a trm" "'a trm" |
+  Lam 'a "'a trm" |
+  Lt "('a \<times> 'a trm) fset" "'a trm"
 
 
-section {* Customization of terms *}
-
-subsection{* Set and map *}
-
-lemma pre_trm_set2_Lt: "pre_trm_set2 (Inr (Inr (Inr (xts, t)))) = snd ` (fset xts) \<union> {t}"
-unfolding pre_trm_set2_def sum_set_defs prod_set_defs collect_def[abs_def]
-by auto
-
-lemma pre_trm_set2_Var: "\<And>x. pre_trm_set2 (Inl x) = {}"
-and pre_trm_set2_App:
-"\<And>t1 t2. pre_trm_set2 (Inr (Inl t1t2)) = {fst t1t2, snd t1t2}"
-and pre_trm_set2_Lam:
-"\<And>x t. pre_trm_set2 (Inr (Inr (Inl (x, t)))) = {t}"
-unfolding pre_trm_set2_def sum_set_defs prod_set_defs collect_def[abs_def]
-by auto
-
-lemma pre_trm_map:
-"\<And> a1. pre_trm_map f1 f2 (Inl a1) = Inl (f1 a1)"
-"\<And> a2 b2. pre_trm_map f1 f2 (Inr (Inl (a2,b2))) = Inr (Inl (f2 a2, f2 b2))"
-"\<And> a1 a2. pre_trm_map f1 f2 (Inr (Inr (Inl (a1,a2)))) = Inr (Inr (Inl (f1 a1, f2 a2)))"
-"\<And> a1a2s a2.
-   pre_trm_map f1 f2 (Inr (Inr (Inr (a1a2s, a2)))) =
-   Inr (Inr (Inr (map_fset (\<lambda> (a1', a2'). (f1 a1', f2 a2')) a1a2s, f2 a2)))"
-unfolding pre_trm_map_def collect_def[abs_def] map_pair_def by auto
-
-
-subsection{* Constructors *}
-
-definition "Var x \<equiv> trm_ctor (Inl x)"
-definition "App t1 t2 \<equiv> trm_ctor (Inr (Inl (t1,t2)))"
-definition "Lam x t \<equiv> trm_ctor (Inr (Inr (Inl (x,t))))"
-definition "Lt xts t \<equiv> trm_ctor (Inr (Inr (Inr (xts,t))))"
-
-lemmas ctor_defs = Var_def App_def Lam_def Lt_def
-
-theorem trm_simps[simp]:
-"\<And>x y. Var x = Var y \<longleftrightarrow> x = y"
-"\<And>t1 t2 t1' t2'. App t1 t2 = App t1' t2' \<longleftrightarrow> t1 = t1' \<and> t2 = t2'"
-"\<And>x x' t t'. Lam x t = Lam x' t' \<longleftrightarrow> x = x' \<and> t = t'"
-"\<And> xts xts' t t'. Lt xts t = Lt xts' t' \<longleftrightarrow> xts = xts' \<and> t = t'"
-(*  *)
-"\<And> x t1 t2. Var x \<noteq> App t1 t2"  "\<And>x y t. Var x \<noteq> Lam y t"  "\<And> x xts t. Var x \<noteq> Lt xts t"
-"\<And> t1 t2 x t. App t1 t2 \<noteq> Lam x t"  "\<And> t1 t2 xts t. App t1 t2 \<noteq> Lt xts t"
-"\<And>x t xts t1. Lam x t \<noteq> Lt xts t1"
-unfolding ctor_defs trm.ctor_inject by auto
-
-theorem trm_cases[elim, case_names Var App Lam Lt]:
-assumes Var: "\<And> x. t = Var x \<Longrightarrow> phi"
-and App: "\<And> t1 t2. t = App t1 t2 \<Longrightarrow> phi"
-and Lam: "\<And> x t1. t = Lam x t1 \<Longrightarrow> phi"
-and Lt: "\<And> xts t1. t = Lt xts t1 \<Longrightarrow> phi"
-shows phi
-proof(cases rule: trm.ctor_exhaust[of t])
-  fix x assume "t = trm_ctor x"
-  thus ?thesis
-  apply(cases x) using Var unfolding ctor_defs apply blast
-  apply(case_tac b) using App unfolding ctor_defs apply(case_tac a, blast)
-  apply(case_tac ba) using Lam unfolding ctor_defs apply(case_tac a, blast)
-  apply(case_tac bb) using Lt unfolding ctor_defs by blast
-qed
+section {* Customi induction rule *}
 
 lemma trm_induct[case_names Var App Lam Lt, induct type: trm]:
-assumes Var: "\<And> (x::'a). phi (Var x)"
+assumes Var: "\<And> x. phi (Var x)"
 and App: "\<And> t1 t2. \<lbrakk>phi t1; phi t2\<rbrakk> \<Longrightarrow> phi (App t1 t2)"
 and Lam: "\<And> x t. phi t \<Longrightarrow> phi (Lam x t)"
 and Lt: "\<And> xts t. \<lbrakk>\<And> x1 t1. (x1,t1) |\<in>| xts \<Longrightarrow> phi t1; phi t\<rbrakk> \<Longrightarrow> phi (Lt xts t)"
 shows "phi t"
-proof(induct rule: trm.ctor_induct)
-  fix u :: "'a + 'a trm \<times> 'a trm + 'a \<times> 'a trm + ('a \<times> 'a trm) fset \<times> 'a trm"
-  assume IH: "\<And>t. t \<in> pre_trm_set2 u \<Longrightarrow> phi t"
-  show "phi (trm_ctor u)"
-  proof(cases u)
-    case (Inl x)
-    show ?thesis using Var unfolding Var_def Inl .
-  next
-    case (Inr uu) note Inr1 = Inr
-    show ?thesis
-    proof(cases uu)
-      case (Inl t1t2)
-      obtain t1 t2 where t1t2: "t1t2 = (t1,t2)" by (cases t1t2, blast)
-      show ?thesis unfolding Inr1 Inl t1t2 App_def[symmetric] apply(rule App)
-      using IH unfolding Inr1 Inl pre_trm_set2_App t1t2 fst_conv snd_conv by blast+
-    next
-      case (Inr uuu) note Inr2 = Inr
-      show ?thesis
-      proof(cases uuu)
-        case (Inl xt)
-        obtain x t where xt: "xt = (x,t)" by (cases xt, blast)
-        show ?thesis unfolding Inr1 Inr2 Inl xt Lam_def[symmetric] apply(rule Lam)
-        using IH unfolding Inr1 Inr2 Inl pre_trm_set2_Lam xt by blast
-      next
-        case (Inr xts_t)
-        obtain xts t where xts_t: "xts_t = (xts,t)" by (cases xts_t, blast)
-        show ?thesis unfolding Inr1 Inr2 Inr xts_t Lt_def[symmetric] apply(rule Lt) using IH
-        unfolding Inr1 Inr2 Inr pre_trm_set2_Lt xts_t fset_fset_member image_def by auto
-      qed
-    qed
-  qed
-qed
-
-
-subsection{* Recursion and iteration (fold) *}
-
-definition
-"sumJoin4 f1 f2 f3 f4 \<equiv>
-\<lambda> k. (case k of
- Inl x1 \<Rightarrow> f1 x1
-|Inr k1 \<Rightarrow> (case k1 of
- Inl ((s2,a2),(t2,b2)) \<Rightarrow> f2 s2 a2 t2 b2
-|Inr k2 \<Rightarrow> (case k2 of Inl (x3,(t3,b3)) \<Rightarrow> f3 x3 t3 b3
-|Inr (xts,(t4,b4)) \<Rightarrow> f4 xts t4 b4)))"
-
-lemma sumJoin4_simps[simp]:
-"\<And>x. sumJoin4 var app lam lt (Inl x) = var x"
-"\<And> t1 a1 t2 a2. sumJoin4 var app lam lt (Inr (Inl ((t1,a1),(t2,a2)))) = app t1 a1 t2 a2"
-"\<And> x t a. sumJoin4 var app lam lt (Inr (Inr (Inl (x,(t,a))))) = lam x t a"
-"\<And> xtas t a. sumJoin4 var app lam lt (Inr (Inr (Inr (xtas,(t,a))))) = lt xtas t a"
-unfolding sumJoin4_def by auto
-
-definition "trmrec var app lam lt \<equiv> trm_ctor_rec (sumJoin4 var app lam lt)"
-
-lemma trmrec_Var[simp]:
-"trmrec var app lam lt (Var x) = var x"
-unfolding trmrec_def Var_def trm.ctor_rec pre_trm_map(1) by simp
-
-lemma trmrec_App[simp]:
-"trmrec var app lam lt (App t1 t2) =
- app t1 (trmrec var app lam lt t1) t2 (trmrec var app lam lt t2)"
-unfolding trmrec_def App_def trm.ctor_rec pre_trm_map(2) convol_def by simp
-
-lemma trmrec_Lam[simp]:
-"trmrec var app lam lt (Lam x t) = lam x t (trmrec var app lam lt t)"
-unfolding trmrec_def Lam_def trm.ctor_rec pre_trm_map(3) convol_def by simp
-
-lemma trmrec_Lt[simp]:
-"trmrec var app lam lt (Lt xts t) =
- lt (map_fset (\<lambda> (x,t). (x,t,trmrec var app lam lt t)) xts) t (trmrec var app lam lt t)"
-unfolding trmrec_def Lt_def trm.ctor_rec pre_trm_map(4) convol_def by simp
-
-definition
-"sumJoinI4 f1 f2 f3 f4 \<equiv>
-\<lambda> k. (case k of
- Inl x1 \<Rightarrow> f1 x1
-|Inr k1 \<Rightarrow> (case k1 of
- Inl (a2,b2) \<Rightarrow> f2 a2 b2
-|Inr k2 \<Rightarrow> (case k2 of Inl (x3,b3) \<Rightarrow> f3 x3 b3
-|Inr (xts,b4) \<Rightarrow> f4 xts b4)))"
-
-lemma sumJoinI4_simps[simp]:
-"\<And>x. sumJoinI4 var app lam lt (Inl x) = var x"
-"\<And> a1 a2. sumJoinI4 var app lam lt (Inr (Inl (a1,a2))) = app a1 a2"
-"\<And> x a. sumJoinI4 var app lam lt (Inr (Inr (Inl (x,a)))) = lam x a"
-"\<And> xtas a. sumJoinI4 var app lam lt (Inr (Inr (Inr (xtas,a)))) = lt xtas a"
-unfolding sumJoinI4_def by auto
-
-(* The iterator has a simpler, hence more manageable type. *)
-definition "trmfold var app lam lt \<equiv> trm_ctor_fold (sumJoinI4 var app lam lt)"
-
-lemma trmfold_Var[simp]:
-"trmfold var app lam lt (Var x) = var x"
-unfolding trmfold_def Var_def trm.ctor_fold pre_trm_map(1) by simp
-
-lemma trmfold_App[simp]:
-"trmfold var app lam lt (App t1 t2) =
- app (trmfold var app lam lt t1) (trmfold var app lam lt t2)"
-unfolding trmfold_def App_def trm.ctor_fold pre_trm_map(2) by simp
-
-lemma trmfold_Lam[simp]:
-"trmfold var app lam lt (Lam x t) = lam x (trmfold var app lam lt t)"
-unfolding trmfold_def Lam_def trm.ctor_fold pre_trm_map(3) by simp
-
-lemma trmfold_Lt[simp]:
-"trmfold var app lam lt (Lt xts t) =
- lt (map_fset (\<lambda> (x,t). (x,trmfold var app lam lt t)) xts) (trmfold var app lam lt t)"
-unfolding trmfold_def Lt_def trm.ctor_fold pre_trm_map(4) by simp
+apply induct
+apply (rule Var)
+apply (erule App, assumption)
+apply (erule Lam)
+using Lt unfolding fset_fset_member mem_Collect_eq
+apply (rule meta_mp)
+defer
+apply assumption
+apply (erule thin_rl)
+apply assumption
+apply (drule meta_spec)
+apply (drule meta_spec)
+apply (drule meta_mp)
+apply assumption
+apply (auto simp: snds_def)
+done
 
 
 subsection{* Example: The set of all variables varsOf and free variables fvarsOf of a term: *}
 
-definition "varsOf = trmfold
+definition "varsOf = trm_fold
 (\<lambda> x. {x})
 (\<lambda> X1 X2. X1 \<union> X2)
 (\<lambda> x X. X \<union> {x})
 (\<lambda> xXs Y. Y \<union> (\<Union> { {x} \<union> X | x X. (x,X) |\<in>| xXs}))"
 
+thm trm.fold
 lemma varsOf_simps[simp]:
 "varsOf (Var x) = {x}"
 "varsOf (App t1 t2) = varsOf t1 \<union> varsOf t2"
 "varsOf (Lam x t) = varsOf t \<union> {x}"
 "varsOf (Lt xts t) =
  varsOf t \<union> (\<Union> { {x} \<union> X | x X. (x,X) |\<in>| map_fset (\<lambda> (x,t1). (x,varsOf t1)) xts})"
-unfolding varsOf_def by simp_all
+unfolding varsOf_def by (simp add: map_pair_def)+
 
-definition "fvarsOf = trmfold
+definition "fvarsOf = trm_fold
 (\<lambda> x. {x})
 (\<lambda> X1 X2. X1 \<union> X2)
 (\<lambda> x X. X - {x})
@@ -225,7 +79,7 @@ lemma fvarsOf_simps[simp]:
  fvarsOf t
  - {x | x X. (x,X) |\<in>| map_fset (\<lambda> (x,t1). (x,fvarsOf t1)) xts}
  \<union> (\<Union> {X | x X. (x,X) |\<in>| map_fset (\<lambda> (x,t1). (x,fvarsOf t1)) xts})"
-unfolding fvarsOf_def by simp_all
+unfolding fvarsOf_def by (simp add: map_pair_def)+
 
 lemma diff_Un_incl_triv: "\<lbrakk>A \<subseteq> D; C \<subseteq> E\<rbrakk> \<Longrightarrow> A - B \<union> C \<subseteq> D \<union> E" by blast
 
